src/Ast/ResolvedPrinter.dfy
@@ -63,6 +63,9 @@ module ResolvedPrinter {
   }
 
   method TypeDecl(decl: TypeDecl, indent: nat) {
+    if decl.FromDomainSignature {
+      print "// ";
+    }
     print "type ", decl.Name, "\n";
   }
 
